Reverse order of arithmetic circuits

code/Decompose.ec
@@ -15,8 +15,8 @@ type input_wires = [
 ].
 
 type gate = [
-  | ADDC of (int * (int -> int))
-  | MULTC of (int * (int -> int))
+  | ADDC of (int * int)
+  | MULTC of (int * int)
   | MULT of (int * int)
   | ADD of (int * int)
 ].
@@ -35,10 +35,10 @@ with g = MULT inputs => let (i, j) = inputs in
 with g = ADD inputs =>  let (i, j) = inputs in
                         let x = (nth 0 s i) in
                         let y = (nth 0 s j) in x + y
-with g = ADDC inputs => let (i, f) = inputs in
-                        let x = (nth 0 s i) in f x
-with g = MULTC inputs => let (i, f) = inputs in
-                         let x = (nth 0 s i) in f x.
+with g = ADDC inputs => let (i, c) = inputs in
+                        let x = (nth 0 s i) in x + c
+with g = MULTC inputs => let (i, c) = inputs in
+                         let x = (nth 0 s i) in x * c.
 
 (* Circuit example: *)
 (* x *)
@@ -48,39 +48,42 @@ with g = MULTC inputs => let (i, f) = inputs in
 (* | / *)
 (* * *)
 
-const circuit_ex = [ADDC (0, fun x => 2 + x); MULT(0,1)].
+const circuit_ex = rev [ADDC (0, 2); MULT(0,1)].
 const s' : state = [10].
 
-op eval_circuit(c : circuit, s : state) : output =
-    with c = [] => last 0 s
-    with c = g :: gs => let r = eval_gate g s in eval_circuit gs (rcons s r).
+(* op eval_circuit(c : circuit, s : state) : output = *)
+(*     with c = [] => last 0 s *)
+(*     with c = g :: gs => let r = eval_gate g s in eval_circuit gs (rcons s r). *)
 
-lemma circuit_ex_test : (eval_circuit circuit_ex [10]) = 120 by trivial.
+op eval_circuit_aux(c : circuit, s : state) : state =
+    with c = [] => s
+    with c = g :: gs =>
+     let s' = eval_circuit_aux gs s in
+     let r = eval_gate g s' in (rcons s' r).
 
-module Tester = {
-  proc main(x : input, c : circuit, s : state) = {
-    return eval_circuit c [x];
-  }
-}.
+op eval_circuit (c : circuit, s : state) : output =
+    last 0 (eval_circuit_aux c s).
 
-lemma test &m:
-    Pr[Tester.main(10, circuit_ex, s') @ &m : res = 120] = 1%r.
-proof. byphoare(: x = 10 /\ c = circuit_ex /\ s = s' ==> _)=>//.
-proc. skip. progress. qed.
+(* lemma eval_circuit_step g gs s: *)
+(*     eval_circuit (g :: gs) s = eval_circuit gs (rcons s (eval_gate g s)). *)
+(* proof. trivial. qed. *)
+
+lemma circuit_ex_test : (eval_circuit circuit_ex [10]) = 120.
+    proof. by rewrite /eval_circuit /circuit_ex /rev /catrev; simplify. qed.
 
 (** Phi protocol **)
 
 (* define decomposed circuit function *)
-op phi_decomp (h : input, g : gate, p : int, w : state list) : output =
+op phi_decomp (g : gate, p : int, w : state list) : output =
 with g = ADDC inputs =>
-    let (i, f) = inputs in
+    let (i, c) = inputs in
     let state = (nth s' w (p - 1)) in
     let x = (nth 0 state i) in
-    if p = 1 then f x else x
+    if p = 1 then x + c else x
 with g = MULTC inputs =>
-    let (i, f) = inputs in
+    let (i, c) = inputs in
     let state = (nth s' w (p - 1)) in
-    let x = (nth 0 state i) in f x
+    let x = (nth 0 state i) in x * c
 with g = ADD inputs =>
     let (i, j) = inputs in
     let state = (nth s' w (p - 1)) in
@@ -97,6 +100,24 @@ with g = MULT inputs =>
     let yp' = (nth 0 statep' j) in
     xp * yp + xp' * yp + xp * yp' + 1 - 1.
 
+op phi_circuit_aux (c : circuit, w1 w2 w3 : view) : (view * view * view) =
+    with c = [] => (w1, w2, w3)
+    with c = g::gs =>
+    let (w1, w2, w3) = phi_circuit_aux gs w1 w2 w3 in
+    let r1 = phi_decomp g 1 [w1;w2;w3] in
+    let r2 = phi_decomp g 2 [w1;w2;w3] in
+    let r3 = phi_decomp g 3 [w1;w2;w3] in
+    (rcons w1 r1, rcons w2 r2, rcons w3 r3).
+
+op phi_circuit (c : circuit, w1, w2, w3 : view) : output =
+    let (w1, w2, w3) = phi_circuit_aux c w1 w2 w3 in
+    last 0 w1 + last 0 w2 + last 0 w3.
+
+
+lemma phi_circuit_ex_test : (phi_circuit circuit_ex [2] [3] [5]) = 120.
+    proof. by rewrite /phi_circuit /circuit_ex /rev. qed.
+
+
 (* secret sharing distribution *)
 op dinput : {input distr | is_lossless dinput /\ is_funiform dinput} as dinput_llfuni.
 
@@ -107,63 +128,196 @@ lemma dinput_fu : is_full dinput by apply/funi_ll_full; [exact/dinput_funi|exact
 (* Random Oracle *)
 
 module Phi = {
-  proc main(x : input, c : circuit) = {
-    var x1, x2, x3, w1, w2, w3, y1, y2, y3, r1, r2, r3;
-    var g : gate;
+  (* proc compute(c : circuit, w1 w2 w3 : view) = { *)
+  (*   var g, r1, r2, r3; *)
+  (*   while (c <> []) { *)
+  (*     g = last (ADDC(0,42)) c; *)
+  (*     r1 = phi_decomp g 1 [w1;w2;w3]; *)
+  (*     r2 = phi_decomp g 2 [w1;w2;w3]; *)
+  (*     r3 = phi_decomp g 3 [w1;w2;w3]; *)
+  (*     w1 = rcons w1 r1; *)
+  (*     w2 = rcons w2 r2; *)
+  (*     w3 = rcons w3 r3; *)
+  (*     c = rev (behead (rev c)); *)
+  (*   } *)
+  (*   return (w1, w2, w3); *)
+  (* } *)
+  (* proc compute_stepped(g : gate, c' : circuit, w1 w2 w3 : view) = { *)
+  (*   (w1, w2, w3) = compute(c', w1, w2, w3); *)
+  (*   (w1, w2, w3) = compute([g], w1, w2, w3); *)
+  (*   return (w1, w2, w3); *)
+  (* } *)
+  proc main(h : input, c : circuit) = {
+    var x1, x2, x3, y;
     x1 <$ dinput;
     x2 <$ dinput;
-    x3 = x - x1 - x2;
-    w1 = [x1];
-    w2 = [x2];
-    w3 = [x3];
-    while (c <> []) {
-      g = head (ADD(0,0)) c;
-      r1 = phi_decomp x g 1 [w1;w2;w3];
-      r2 = phi_decomp x g 2 [w1;w2;w3];
-      r3 = phi_decomp x g 3 [w1;w2;w3];
-      w1 = rcons w1 r1;
-      w2 = rcons w2 r2;
-      w3 = rcons w3 r3;
-      c = behead c;
-    }
-    y1 = last 0 w1;
-    y2 = last 0 w2;
-    y3 = last 0 w3;
-    (* return (w1, w2, w3, y1, y2, y3); *)
-    return y1 + y2 + y3;
+    x3 = h - x1 - x2;
+    y = phi_circuit c [x1] [x2] [x3];
+    return y;
   }
 }.
 
 lemma decomp_test &m:
     Pr[Phi.main(10, circuit_ex) @ &m : res = 120] = 1%r.
 proof.
-    byphoare(: x = 10 /\ c = circuit_ex ==> _)=>//.
+    byphoare(: h = 10 /\ c = circuit_ex ==> _)=>//.
     proc. auto.
-    seq 3 : (x = x1 + x2 + x3 /\ #pre). auto. auto. progress. apply dinput_ll. algebra.
-    sp. rewrite /circuit_ex.
-    rcondt 1. auto.
-    sp. elim*. progress.
-    rcondt 1. auto.
-    sp. elim*. progress.
-    rcondf 1. auto.
-    auto. progress.
-    smt().
-    hoare. auto. progress. algebra. progress.
+    rewrite /circuit_ex /rev. progress.
+    apply dinput_ll.
+    rewrite /phi_circuit /rev. simplify. algebra.
 qed.
 
-lemma decompo_circuit_equiv &m x':
+lemma decompo_circuit_ex_equiv &m x':
     Pr[Phi.main(x', circuit_ex) @ &m : res = eval_circuit circuit_ex [x'] ] = 1%r.
 proof.
-    byphoare(: x = x' /\ c = circuit_ex ==> _)=>//.
+    byphoare(: h = x' /\ c = circuit_ex ==> _)=>//.
+    proc.  auto.
+    rewrite /circuit_ex /rev. progress.
+    apply dinput_ll.
+    rewrite /eval_circuit /phi_circuit /rev. simplify. algebra.
+qed.
+
+lemma decomp_equiv_ind g gs (x x1 x2 x3 : input) (w1 w2 w3 : view) r1 r2 r3:
+    r1 = phi_decomp g 1 [w1;w2;w3] /\
+    r2 = phi_decomp g 2 [w1;w2;w3] /\
+    r3 = phi_decomp g 3 [w1;w2;w3] =>
+    ((rcons w1 r1), (rcons w2 r2), (rcons w3 r3)) = phi_circuit_aux (g::gs) [x1] [x2] [x3]
+    <=> (w1, w2, w3) = phi_circuit_aux gs [x1] [x2] [x3].
+proof.
+  progress.
+  - smt.
+  - elim g; progress; rewrite - H.
+    + elim x0; progress. smt().
+    + elim x0; progress. smt().
+qed.
+
+lemma circuit_equiv_ind g gs (x : input) s r:
+    r = eval_gate g s =>
+    (rcons s r) = eval_circuit_aux (g::gs) [x]
+    <=> s = eval_circuit_aux gs [x].
+proof.
+  progress. smt.
+qed.
+
+lemma decomp_equiv g (x x1 x2 x3 : input) (w1 w2 w3 : view) s:
+    (x = x1 + x2 + x3 /\ (w1, w2, w3) = phi_circuit_aux [g] [x1] [x2] [x3] /\
+    s = eval_circuit_aux [g] [x]) =>
+    (forall i, (nth 0 w1 i) + (nth 0 w2 i) + (nth 0 w3 i) = (nth 0 s i)).
+proof.
+  elim g; progress.
+  - smt().
+  - smt().
+  - elim x0=> x01 x02; case (i = 0); case (i - 1 = 0); case (x01 = 0); case(x02 = 0); progress.
+    algebra. case (x02 = 0). progress. algebra. progress. case (x01 = 0). progress. algebra.
+    progress. case (x01 = 0); case (x02 = 0); progress. algebra.
+  - elim x0=> x01 x02; case (i = 0); case (i - 1 = 0); case (x01 = 0); case(x02 = 0); progress.
+    algebra. case (x02 = 0). progress. algebra. progress. case (x01 = 0). progress. algebra.
+    progress. case (x01 = 0); case (x02 = 0); progress. algebra.
+qed.
+
+lemma decomp_equiv_ind gs (x x1 x2 x3 : input) (w1 w2 w3 : view) s:
+    (x = x1 + x2 + x3 /\ (w1, w2, w3) = phi_circuit_aux gs [x1] [x2] [x3] /\
+    s = eval_circuit_aux gs [x]) =>
+    (forall i, (nth 0 w1 i) + (nth 0 w2 i) + (nth 0 w3 i) = (nth 0 s i)).
+proof.
+   elim gs; progress. smt().
+   have : (w1, w2, w3) = phi_circuit_aux (x0::l) [x1] [x2] [x3].
+   smt.
+   clear H0.
+   have -> : (rcons (eval_circuit_aux l [x1 + x2 + x3]) (eval_gate x0 (eval_circuit_aux l [x1 + x2 + x3]))) = eval_circuit_aux (x0::l) [x1+x2+x3].
+   smt.
+   move=> H1.
+   progress.
+   smt.
+
+
+lemma decompo_circuit_ex_equiv &m x' c':
+    Pr[Phi.main(x', c') @ &m : res = eval_circuit c' [x'] ] = 1%r.
+proof.
+    elim c'.
+    byphoare(: h = x' /\ c = [] ==> _)=>//.
+    proc.  auto.
+    rewrite /circuit_ex /rev. progress.
+    apply dinput_ll.
+    rewrite /eval_circuit /phi_circuit /rev. simplify.
+    algebra.
+    progress.
+    byphoare(: h = x' /\ c = (x::l) ==> _)=>//.
     proc. auto.
-    seq 3 : (x = x1 + x2 + x3 /\ #pre). auto. auto. progress. apply dinput_ll. algebra.
-    sp. rewrite /circuit_ex.
-    rcondt 1. auto.
-    sp. elim*. progress.
-    rcondt 1. auto.
-    sp. elim*. progress.
-    rcondf 1. auto.
-    auto. progress.
+    rewrite /circuit_ex /rev. progress.
+    apply dinput_ll.
+qed.
+
+
+lemma decomp_gate_equiv g w1' w2' w3' s':
+    (forall i, (nth 0 w1' i) + (nth 0 w2' i) + (nth 0 w3' i) = (nth 0 s' i)) =>
+    phoare[Phi.compute : (c = [g] /\ w1 = w1' /\ w2 = w2' /\ w3 = w3' )
+            ==> let (w1, w2, w3) = res in last 0 w1 + last 0 w2 + last 0 w3 = eval_circuit [g] s'] = 1%r.
+proof.
+  move=> invariant.
+  proc. inline *. wp.
+  rcondt 1. auto.
+  sp. elim*. auto.
+  rcondf 1. auto.
+  elim g; rewrite /rev; progress.
+  elim g; rewrite /rev; auto; progress.
+  - case x. progress.
+    rewrite /rcons /last /eval_circuit. simplify.
+    rewrite !last_rcons.
+    rewrite - invariant.
+    algebra.
+  - case x. progress.
+    rewrite /rcons /last /eval_circuit. simplify.
+    rewrite !last_rcons.
+    rewrite - invariant.
+    algebra.
+  - case x. progress.
+    rewrite /rcons /last /eval_circuit. simplify.
+    rewrite !last_rcons.
+    rewrite - invariant.
     smt().
-    hoare. auto. progress. algebra. progress.
+  - case x. progress.
+    rewrite /rcons /last /eval_circuit. simplify.
+    rewrite !last_rcons.
+    rewrite - invariant.
+    smt().
+qed.
+
+lemma decomp_gate_equiv &m c' (x1 x2 x3 : input):
+    (* (forall i, (nth 0 w1' i) + (nth 0 w2' i) + (nth 0 w3' i) = (nth 0 s' i)) => *)
+    phoare[Phi.compute : (c = c' /\ w1 = [x1] /\ w2 = [x2] /\ w3 = [x3] )
+      ==> let (w1, w2, w3) = res in
+          let s = eval_circuit_aux c' [x1 + x2 + x3] in
+            (forall i, (nth 0 w1 i) + (nth 0 w2 i) + (nth 0 w3 i) = (nth 0 s i))] = 1%r.
+proof.
+    elim c'.
+    proc.  rcondf 1. auto. auto. progress. smt().
+    progress.
+
+lemma compute_circuit_equiv &m x' g c':
+    phoare[Phi.compute : (x = x' /\ c = c') ==>
+      let (w1, w2, w3) = res in last 0 w1 + last 0 w2 + last 0 w3 = eval_circuit c' [x']] = 1%r =>
+    phoare[Phi.compute : (x = x' /\ c = (g::c')) ==>
+      let (w1, w2, w3) = res in last 0 w1 + last 0 w2 + last 0 w3 = eval_circuit (g::c') [x']] = 1%r.
+proof. move=> H.
+   proc. unroll 1.
+   rcondt 1. auto.
+   sp. elim*. progress.
+   conseq H.
+
+
+lemma decompo_circuit_equiv &m x' c':
+    phoare[Phi.main : (x = x' /\ c = c') ==> res = eval_circuit c' [x']] = 1%r.
+proof.
+  proc. auto.
+  seq 3 : (x = x1 + x2 + x3 /\ #pre). auto. auto. progress. apply dinput_ll. algebra.
+  exists* x1. exists* x2. exists* x3. elim*=> x1 x2 x3.
+  call (: w1 = [x1] /\ w2 = [x2] /\ w3 =  [x3] /\ x' = x1 + x2 + x3 /\ c = c' ==> let (w1, w2, w3) = res in last 0 w1 + last 0 w2 + last 0 w3 = eval_circuit c' [x']).
+  proc. elim c'.
+  (* call (: Phi.w1 = x1 + x2 + x3). elim c'. *)
+  * rcondf 1; auto.
+  * progress. rcondt 1. auto.
+    sp. elim*. auto. admit.
+  * hoare. auto. progress. algebra.
+  * progress.
 qed.
